units of rates

AwesomeDashboards/NodeExporter.lean
@@ -14,18 +14,35 @@ def node_filesystem_avail_bytes : Metric := {
   unit := MetricUnit.bytes
 }
 
+def process_cpu_seconds_total : Metric := {
+  name := "process_cpu_seconds_total"
+  type := MetricType.counter
+  labels := []
+  unit := MetricUnit.seconds
+}
+
+def node_network_receive_bytes_total : Metric := {
+  name := "node_network_receive_bytes_total"
+  type := MetricType.counter
+  labels := ["device"]
+  unit := MetricUnit.bytes
+}
+
 def node_exporter : Exporter := {
-  metrics := [node_boot_time_seconds, node_filesystem_avail_bytes]
+  metrics := [node_boot_time_seconds, node_filesystem_avail_bytes, process_cpu_seconds_total, node_network_receive_bytes_total]
 }
 
 def lm : List KeyValuePair := [{key := "__name__", value := "node_filesystem_avail_bytes"}]
-def v := InstantVector.selector lm 0
+def v := InstantVector.selector {equal := lm} 0
 
 #eval InstantVector.typesafe v node_exporter
 #eval List.map (λ l => l.key) (lm.filter $ is_name)
 #eval List.all (lm.filter $ is_name) (λ l => "node_filesystem_avail_bytes" = l.key )
 
-example : InstantVector.typesafe (InstantVector.selector [{key := "__name__", value := "node_filesystem_avail_bytes"}] 0) node_exporter := by simp
+example : InstantVector.typesafe (InstantVector.selector {equal := lm} 0) node_exporter := by simp
 
 def avail_bytes : InstantVector InstantVectorType.vector := [pql| node_filesystem_avail_bytes-node_filesystem_avail_bytes]
 #eval unitOf node_exporter avail_bytes
+#eval RangeVector.unitOf node_exporter $ RangeVector.selector (LabelMatchers.empty.withName "node_network_receive_bytes_total") 5
+#eval unitOf node_exporter [pql| rate(node_network_receive_bytes_total{}[5])]
+#eval [pql| rate(node_network_receive_bytes_total{device="vda"}[120])]
