Main.lean
@@ -4,11 +4,12 @@ import AwesomeDashboards.Prometheus
 import Lean.Data.Json
 
 def myDashboard : Dashboard node_exporter := { name := "My Dashboard", panels := [
-    (Panel.graph { bottomY := 0, topY := 0, promql := { v := [pql| node_filesystem_avail_bytes{}] } }),
-    (Panel.graph { bottomY := 0, topY := 0, promql := { v := [pql| node_filesystem_avail_bytes] } }),
+    (Panel.graph { promql := { v := [pql| node_filesystem_avail_bytes{}] } }),
+    (Panel.graph { promql := { v := [pql| process_cpu_seconds_total] } }),
+    (Panel.graph { promql := { v := [pql| rate(node_network_receive_bytes_total{device="eth0"}[120])] } }),
     (Panel.table { name := "", columns := [
-      { name := "Uptime", data := (ColumnValueSource.PrometheusValueColumn $ InstantVector.selector [{key := "__name__", value := "node_boot_time_seconds"}] 0), index_label := "instance" },
-      { name := "Free disk space", data := (ColumnValueSource.PrometheusValueColumn $ InstantVector.selector [{key := "__name__", value := "node_filesystem_avail_bytes"}] 0), index_label := "instance" }
+      { name := "Uptime", data := (ColumnValueSource.PrometheusValueColumn [pql| node_boot_time_seconds]), index_label := "instance" },
+      { name := "Free disk space", data := (ColumnValueSource.PrometheusValueColumn [pql| node_filesystem_avail_bytes]), index_label := "instance" }
     ] })
   ] }
 
